Only pure steps in lifting.v

theories/progLog2.v
@@ -1,472 +1,112 @@
 From iris.proofmode Require Import proofmode.
 From iris.base_logic Require Export invariants gen_heap.
-From iris.program_logic Require Export weakestpre ectx_lifting.
+From iris.program_logic Require Export weakestpre ectx_lifting total_weakestpre.
 From iris.algebra Require Import frac auth gmap excl.
 From Coq.Lists Require Import List.
 From ASMinCoq Require Import CpdtTactics.
-From ASMinCoq Require Import AsmGen.
+From ASMinCoq Require Import AsmGen progLog.
 
-
-(* CMRA for invariants *)
-Class invG Σ := InvG {
-  inv_invG : invGS Σ;}.
-
-(* CMRΑ for memory *)
-Class mem1G Σ := Mem1G {
-  mem_gen_mem1G :: gen_heapGS Addr Word Σ}.
-
-Class mem2G Σ := Mem2G {
-  mem_gen_mem2G :: gen_heapGS Addr Word Σ}.
-
-(* CMRA for registers *)
-Class reg1G Σ := Reg1G {
-  reg_gen_reg1G :: gen_heapGS Reg Word Σ; }.
-
-Class reg2G Σ := Reg2G {
-  reg_gen_reg2G :: gen_heapGS Reg Word Σ; }.
-
-
-(* Stuff for the trace copied from Katamaran *)
-Class trace1G (Trace : Type) Σ := Trace1G {
-    trace1_inG :: inG Σ (authR (optionUR (exclR (leibnizO Trace))));
-    trace1_name : gname
+Class binDG Σ := BinDG {
+  bin_invG :> invGS Σ;
+  fst_memG :> gen_heapGS Addr Word Σ;
+  snd_memG :> gen_heapGS Addr Word Σ;
+  fst_regG :> gen_heapGS Register Word Σ;
+  snd_regG :> gen_heapGS Register Word Σ;
+  fst_traceG :: traceG (list leak) Σ;
+  fst_pcG :: traceG Word Σ;
+  fst_progG :: traceG program Σ;
+  snd_traceG :: traceG (list leak) Σ;
+  snd_pcG :: traceG Word Σ;
+  snd_progG :: traceG program Σ;
 }.
-
-Class trace2G (Trace : Type) Σ := Trace2G {
-    trace2_inG :: inG Σ (authR (optionUR (exclR (leibnizO Trace))));
-    trace2_name : gname
-}.
-
-Definition trace1PreΣ (Trace : Type) : gFunctors := #[GFunctor (authR (optionUR (exclR (leibnizO Trace))))].
-Definition trace2PreΣ (Trace : Type) : gFunctors := #[GFunctor (authR (optionUR (exclR (leibnizO Trace))))].
-
-Class trace1_preG (Trace : Type) Σ := {
-  trace1_preG_inG :: inG Σ (authR (optionUR (exclR (leibnizO Trace))));
-}.
-
-Class trace2_preG (Trace : Type) Σ := {
-  trace2_preG_inG :: inG Σ (authR (optionUR (exclR (leibnizO Trace))));
-}.
-
-#[export] Instance trace1G_preG `{trace1G T Σ} : trace1_preG T Σ.
-Proof. constructor. typeclasses eauto. Defined.
-
-#[export] Instance trace2G_preG `{trace2G T Σ} : trace2_preG T Σ.
-Proof. constructor. typeclasses eauto. Defined.
-
-#[export] Instance subG_trace1PreΣ {Σ T}:
-  subG (trace1PreΣ T) Σ →
-  trace1_preG T Σ.
-Proof. solve_inG. Qed.
-
-#[export] Instance subG_trace2PreΣ {Σ T}:
-  subG (trace2PreΣ T) Σ →
-  trace2_preG T Σ.
-Proof. solve_inG. Qed.
-
-
-Section S.
-  Context `{!trace1_preG T Σ}.
-  Context (γ : gname).
-
-  Definition tr1_auth (t : T) : iProp Σ := own γ  (● (Some (Excl (t : leibnizO T)))).
-  Definition tr1_frag (t : T) : iProp Σ := own γ (◯ (Some (Excl (t : leibnizO T)))).
-
-  Lemma trace1_full_frag_eq t t':
-    tr1_auth t -∗ tr1_frag t' -∗
-    ⌜ t = t' ⌝.
-  Proof.
-    iIntros "H1 H2".
-    iDestruct (own_valid_2 with "H1 H2") as %[Hi Hv]%auth_both_valid_discrete.
-    rewrite Excl_included in Hi.  apply leibniz_equiv in Hi. subst; auto.
-  Qed.
-
-  Lemma tr1_frag_excl t t' :
-    tr1_frag t -∗ tr1_frag t' -∗ ⌜ False ⌝.
-  Proof.
-    iIntros "H1 H2". iDestruct (own_valid_2 with "H1 H2") as %Hv.
-    now apply excl_auth.excl_auth_frag_op_valid in Hv.
-  Qed.
-
-  Lemma trace1_update t t' :
-    tr1_auth t ∗ tr1_frag t ==∗
-    tr1_auth t' ∗ tr1_frag t'.
-  Proof.
-    rewrite /tr1_auth /tr1_frag. rewrite -!own_op.
-    iApply own_update. apply auth_update.
-    apply option_local_update.
-    apply exclusive_local_update. constructor.
-  Qed.
-
-  (* For the moment, there is no need for a lemma stating that traces can only be appened to, but we could customize the RA to enforce this. *)
-
-  #[export] Instance tr1_auth_Timeless t : Timeless (tr1_auth t).
-  Proof.
-    intros. apply _.
-  Qed.
-
-  #[export] Instance tr1_frag_Timeless t : Timeless (tr1_frag t).
-  Proof.
-    intros. apply _.
-  Qed.
-End S.
-
-Section S.
-  Context `{!trace2_preG T Σ}.
-  Context (γ : gname).
-
-  Definition tr2_auth (t : T) : iProp Σ := own γ (● (Some (Excl (t : leibnizO T)))).
-  Definition tr2_frag (t : T) : iProp Σ := own γ (◯ (Some (Excl (t : leibnizO T)))).
-
-  Lemma trace2_full_frag_eq t t':
-    tr2_auth t -∗ tr2_frag t' -∗
-    ⌜ t = t' ⌝.
-  Proof.
-    iIntros "H1 H2".
-    iDestruct (own_valid_2 with "H1 H2") as %[Hi Hv]%auth_both_valid_discrete.
-    rewrite Excl_included in Hi.  apply leibniz_equiv in Hi. subst; auto.
-  Qed.
-
-  Lemma tr2_frag_excl t t' :
-    tr2_frag t -∗ tr2_frag t' -∗ ⌜ False ⌝.
-  Proof.
-    iIntros "H1 H2". iDestruct (own_valid_2 with "H1 H2") as %Hv.
-    now apply excl_auth.excl_auth_frag_op_valid in Hv.
-  Qed.
-
-  Lemma trace2_update t t' :
-    tr2_auth t ∗ tr2_frag t ==∗
-    tr2_auth t' ∗ tr2_frag t'.
-  Proof.
-    rewrite /tr2_auth /tr2_frag. rewrite -!own_op.
-    iApply own_update. apply auth_update.
-    apply option_local_update.
-    apply exclusive_local_update. constructor.
-  Qed.
-
-  (* For the moment, there is no need for a lemma stating that traces can only be appened to, but we could customize the RA to enforce this. *)
-
-  #[export] Instance tr2_auth_Timeless t : Timeless (tr2_auth t).
-  Proof.
-    intros. apply _.
-  Qed.
-
-  #[export] Instance tr2_frag_Timeless t : Timeless (tr2_frag t).
-  Proof.
-    intros. apply _.
-  Qed.
-End S.
-
-(* Stuff for the PC *)
-Class pc1G Σ := Pc1G {
-    pc1_inG :: inG Σ (authR (optionUR (exclR (leibnizO Word))));
-    pc1_name : gname
-}.
-
-Class pc2G Σ := Pc2G {
-    pc2_inG :: inG Σ (authR (optionUR (exclR (leibnizO Word))));
-    pc2_name : gname
-}.
-
-Definition Pc1PreΣ : gFunctors := #[GFunctor (authR (optionUR (exclR (leibnizO 
-Word))))].
-
-Definition Pc2PreΣ : gFunctors := #[GFunctor (authR (optionUR (exclR (leibnizO 
-Word))))].
-
-Class PC1_preG Σ := {
-  PC1_preG_inG :: inG Σ (authR (optionUR (exclR (leibnizO Word))));
-}.
-
-Class PC2_preG Σ := {
-  PC2_preG_inG :: inG Σ (authR (optionUR (exclR (leibnizO Word))));
-}.
-
-#[export] Instance Pc1G_preG `{pc1G Σ} : PC1_preG Σ.
-Proof. constructor. typeclasses eauto. Defined.
-
-#[export] Instance Pc2G_preG `{pc2G Σ} : PC2_preG Σ.
-Proof. constructor. typeclasses eauto. Defined.
-
-#[export] Instance subG_Pc1PreΣ {Σ}:
-  subG Pc1PreΣ Σ →
-  PC1_preG Σ.
-Proof. solve_inG. Qed.
-
-#[export] Instance subG_Pc2PreΣ {Σ}:
-  subG Pc2PreΣ Σ →
-  PC2_preG Σ.
-Proof. solve_inG. Qed.
-
-Section S.
-  Context `{!pc1G Σ}.
-  Context (γ : gname).
-
-  Definition pc1_auth (w : Word) : iProp Σ := own γ (● (Some (Excl (w : leibnizO Word)))).
-  Definition pc1_frag (w : Word) : iProp Σ := own γ (◯ (Some (Excl (w : leibnizO Word)))).
-
-  Lemma pc1_full_frag_eq t t':
-    pc1_auth t -∗ pc1_frag t' -∗
-    ⌜ t = t' ⌝.
-  Proof.
-    iIntros "H1 H2".
-    iDestruct (own_valid_2 with "H1 H2") as %[Hi Hv]%auth_both_valid_discrete.
-    rewrite Excl_included in Hi. apply leibniz_equiv in Hi. subst; auto.
-  Qed.
-
-  Lemma pc1_frag_excl t t' :
-    pc1_frag t -∗ pc1_frag t' -∗ ⌜ False ⌝.
-  Proof.
-    iIntros "H1 H2". iDestruct (own_valid_2 with "H1 H2") as %Hv.
-    now apply excl_auth.excl_auth_frag_op_valid in Hv.
-  Qed.
-
-  Lemma pc1_update t t' :
-    pc1_auth t ∗ pc1_frag t ==∗
-    pc1_auth t' ∗ pc1_frag t'.
-  Proof.
-    rewrite /pc1_auth /pc1_frag. rewrite -!own_op.
-    iApply own_update. apply auth_update.
-    apply option_local_update.
-    apply exclusive_local_update. constructor.
-  Qed.
-
-  (* For the moment, there is no need for a lemma stating that traces can only be appened to, but we could customize the RA to enforce this. *)
-
-  #[export] Instance pc1_auth_Timeless t : Timeless (pc1_auth t).
-  Proof.
-    intros. apply _.
-  Qed.
-
-  #[export] Instance pc1_frag_Timeless t : Timeless (pc1_frag t).
-  Proof.
-    intros. apply _.
-  Qed.
-End S.
-
-Section S.
-  Context `{!pc2G Σ}.
-  Context (γ : gname).
-
-  Definition pc2_auth (w : Word) : iProp Σ := own γ (● (Some (Excl (w : leibnizO Word)))).
-  Definition pc2_frag (w : Word) : iProp Σ := own γ (◯ (Some (Excl (w : leibnizO Word)))).
-
-  Lemma pc2_full_frag_eq t t':
-    pc2_auth t -∗ pc2_frag t' -∗
-    ⌜ t = t' ⌝.
-  Proof.
-    iIntros "H1 H2".
-    iDestruct (own_valid_2 with "H1 H2") as %[Hi Hv]%auth_both_valid_discrete.
-    rewrite Excl_included in Hi. apply leibniz_equiv in Hi. subst; auto.
-  Qed.
-
-  Lemma pc2_frag_excl t t' :
-    pc2_frag t -∗ pc2_frag t' -∗ ⌜ False ⌝.
-  Proof.
-    iIntros "H1 H2". iDestruct (own_valid_2 with "H1 H2") as %Hv.
-    now apply excl_auth.excl_auth_frag_op_valid in Hv.
-  Qed.
-
-  Lemma pc2_update t t' :
-    pc2_auth t ∗ pc2_frag t ==∗
-    pc2_auth t' ∗ pc2_frag t'.
-  Proof.
-    rewrite /pc2_auth /pc2_frag. rewrite -!own_op.
-    iApply own_update. apply auth_update.
-    apply option_local_update.
-    apply exclusive_local_update. constructor.
-  Qed.
-
-  (* For the moment, there is no need for a lemma stating that traces can only be appened to, but we could customize the RA to enforce this. *)
-
-  #[export] Instance pc2_auth_Timeless t : Timeless (pc2_auth t).
-  Proof.
-    intros. apply _.
-  Qed.
-
-  #[export] Instance pc2_frag_Timeless t : Timeless (pc2_frag t).
-  Proof.
-    intros. apply _.
-  Qed.
-End S.
-
-(* Stuff for the prog *)
-Class program1G Σ := Program1G {
-    program1_inG :: inG Σ (authR (optionUR (exclR (leibnizO program))));
-    program1_name : gname
-}.
-
-Class program2G Σ := Program2G {
-    program2_inG :: inG Σ (authR (optionUR (exclR (leibnizO program))));
-    program2_name : gname
-}.
-
-Definition Program1PreΣ : gFunctors := #[GFunctor (authR (optionUR (exclR (leibnizO program))))].
-Definition Program2PreΣ : gFunctors := #[GFunctor (authR (optionUR (exclR (leibnizO program))))].
-
-Class Program1_preG Σ := {
-  Program1_preG_inG :: inG Σ (authR (optionUR (exclR (leibnizO program))));
-}.
-
-Class Program2_preG Σ := {
-  Program2_preG_inG :: inG Σ (authR (optionUR (exclR (leibnizO program))));
-}.
-
-#[export] Instance Program1G_preG `{program1G Σ} : Program1_preG Σ.
-Proof. constructor. typeclasses eauto. Defined.
-
-#[export] Instance Program2G_preG `{program2G Σ} : Program2_preG Σ.
-Proof. constructor. typeclasses eauto. Defined.
-
-#[export] Instance subG_Program1PreΣ {Σ}:
-  subG Program1PreΣ Σ →
-  Program1_preG Σ.
-Proof. solve_inG. Qed.
-
-#[export] Instance subG_Program2PreΣ {Σ}:
-  subG Program2PreΣ Σ →
-  Program2_preG Σ.
-Proof. solve_inG. Qed.
-
-Section S.
-  Context `{!program1G Σ}.
-  Context (γ : gname).
-
-  Definition program1_auth (p : program) : iProp Σ := own γ (● (Some (Excl (p : leibnizO program)))).
-  Definition program1_frag (p : program) : iProp Σ := own γ (◯ (Some (Excl (p : leibnizO program)))).
-
-  Lemma program1_full_frag_eq t t':
-    program1_auth t -∗ program1_frag t' -∗
-    ⌜ t = t' ⌝.
-  Proof.
-    iIntros "H1 H2".
-    iDestruct (own_valid_2 with "H1 H2") as %[Hi Hv]%auth_both_valid_discrete.
-    rewrite Excl_included in Hi. apply leibniz_equiv in Hi. subst; auto.
-  Qed.
-
-  Lemma program1_frag_excl t t' :
-    program1_frag t -∗ program1_frag t' -∗ ⌜ False ⌝.
-  Proof.
-    iIntros "H1 H2". iDestruct (own_valid_2 with "H1 H2") as %Hv.
-    now apply excl_auth.excl_auth_frag_op_valid in Hv.
-  Qed.
-
-  Lemma program1_update t t' :
-    program1_auth t ∗ program1_frag t ==∗
-    program1_auth t' ∗ program1_frag t'.
-  Proof.
-    rewrite /program1_auth /program1_frag. rewrite -!own_op.
-    iApply own_update. apply auth_update.
-    apply option_local_update.
-    apply exclusive_local_update. constructor.
-  Qed.
-
-  (* For the moment, there is no need for a lemma stating that traces can only be appened to, but we could customize the RA to enforce this. *)
-
-  #[export] Instance program1_auth_Timeless t : Timeless (program1_auth t).
-  Proof.
-    intros. apply _.
-  Qed.
-
-  #[export] Instance program1_frag_Timeless t : Timeless (program1_frag t).
-  Proof.
-    intros. apply _.
-  Qed.
-End S.
-
-Section S.
-  Context `{!program2G Σ}.
-  Context (γ : gname).
-
-  Definition program2_auth (p : program) : iProp Σ := own γ (● (Some (Excl (p : leibnizO program)))).
-  Definition program2_frag (p : program) : iProp Σ := own γ (◯ (Some (Excl (p : leibnizO program)))).
-
-  Lemma program2_full_frag_eq t t':
-    program2_auth t -∗ program2_frag t' -∗
-    ⌜ t = t' ⌝.
-  Proof.
-    iIntros "H1 H2".
-    iDestruct (own_valid_2 with "H1 H2") as %[Hi Hv]%auth_both_valid_discrete.
-    rewrite Excl_included in Hi. apply leibniz_equiv in Hi. subst; auto.
-  Qed.
-
-  Lemma program2_frag_excl t t' :
-    program2_frag t -∗ program2_frag t' -∗ ⌜ False ⌝.
-  Proof.
-    iIntros "H1 H2". iDestruct (own_valid_2 with "H1 H2") as %Hv.
-    now apply excl_auth.excl_auth_frag_op_valid in Hv.
-  Qed.
-
-  Lemma program2_update t t' :
-    program2_auth t ∗ program2_frag t ==∗
-    program2_auth t' ∗ program2_frag t'.
-  Proof.
-    rewrite /program2_auth /program2_frag. rewrite -!own_op.
-    iApply own_update. apply auth_update.
-    apply option_local_update.
-    apply exclusive_local_update. constructor.
-  Qed.
-
-  (* For the moment, there is no need for a lemma stating that traces can only be appened to, but we could customize the RA to enforce this. *)
-
-  #[export] Instance program2_auth_Timeless t : Timeless (program2_auth t).
-  Proof.
-    intros. apply _.
-  Qed.
-
-  #[export] Instance program2_frag_Timeless t : Timeless (program2_frag t).
-  Proof.
-    intros. apply _.
-  Qed.
-End S.
-
-(* A lot of duplication for the resources right now.
-   Since only 2 types of resources are used heaps (with gen_heap_interp)
-   and exclusive (with copy paste for Katamaran),
-   it should be possible to get rid of most copy paste.
-  *)
-
 
 (* invariants for memory, and a state interpretation for (mem,reg) *)
-Global Instance memG_irisG
-  `{!invG Σ,
-    !mem1G Σ, !reg1G Σ, !trace1G (list leak) Σ, !pc1G Σ, !program1G Σ,
-    !mem2G Σ, !reg2G Σ, !trace2G (list leak) Σ, !pc2G Σ, !program2G Σ
-} : irisGS asm_lang2 Σ
-      := {
-  iris_invGS := inv_invG;
-  state_interp σ _ κs _ :=
-    ((gen_heap_interp (reg σ.1.1.2)) ∗
-    (gen_heap_interp (mem σ.1.1.2)) ∗
-    tr1_auth trace1_name σ.1.2 ∗ pc1_auth pc1_name (PC σ.1.1.2) ∗
-    program1_auth program1_name σ.1.1.1
-    ∗
-    (gen_heap_interp (reg σ.2.1.2)) ∗
-    (gen_heap_interp (mem σ.2.1.2)) ∗
-    tr2_auth trace2_name σ.2.2 ∗ pc2_auth pc2_name (PC σ.2.1.2) ∗
-    program2_auth program2_name σ.2.1.1)%I;
-  fork_post _ := False%I;
-  num_laters_per_step _ := 0;
-  state_interp_mono _ _ _ _ := fupd_intro _ _
-}.
+Global Instance irisG1 `{!binDG Σ} : irisGS asm_lang Σ := {
+    iris_invGS := bin_invG;
+    state_interp σ _ κs _ :=
+      ((@gen_heap_interp _ _ _ _ _ fst_regG (reg σ.1.2)) ∗
+         (@gen_heap_interp _ _ _ _ _ fst_memG (mem σ.1.2)) ∗
+         @tr_auth _ _ fst_traceG σ.2 ∗
+         @tr_auth _ _ fst_pcG (PC σ.1.2) ∗
+         @tr_auth _ _ fst_progG σ.1.1)%I;
+    fork_post _ := False%I;
+    num_laters_per_step _ := 0;
+    state_interp_mono _ _ _ _ := fupd_intro _ _
+  }.
+
+Global Instance irisG2 `{!binDG Σ} : irisGS asm_lang Σ := {
+    iris_invGS := bin_invG;
+    state_interp σ _ κs _ :=
+      ((@gen_heap_interp _ _ _ _ _ snd_regG (reg σ.1.2)) ∗
+         (@gen_heap_interp _ _ _ _ _ snd_memG (mem σ.1.2)) ∗
+         @tr_auth _ _ snd_traceG σ.2 ∗
+         @tr_auth _ _ snd_pcG (PC σ.1.2) ∗
+         @tr_auth _ _ snd_progG σ.1.1)%I;
+    fork_post _ := False%I;
+    num_laters_per_step _ := 0;
+    state_interp_mono _ _ _ _ := fupd_intro _ _
+  }.
+
+Definition TWP1 `{!binDG Σ} (e : expr) (E : coPset) (R : val → iProp Σ) :=
+  @twp (iProp Σ) expr val stuckness
+    (@twp' _ asm_lang Σ irisG1)
+    NotStuck E e R.
+
+Definition TWP2 `{!binDG Σ} (e : expr) (E : coPset) (R : val → iProp Σ) :=
+  @twp (iProp Σ) expr val stuckness
+    (@twp' _ asm_lang Σ irisG2)
+    NotStuck E e R.
 
 Section asm_lang_rules.
-  Context `{!invG Σ,
-  !mem1G Σ, !reg1G Σ, !trace1G (list leak) Σ, !pc1G Σ, !program1G Σ,
-  !mem2G Σ, !reg2G Σ, !trace2G (list leak) Σ, !pc2G Σ, !program2G Σ
-}.
+  Context `{!binDG Σ}.
   Context (γ ζ ξ : gname).
 (* Points to predicates for registers *)
-Notation "r ↦ᵣ{ q } w" := (mapsto (L:=Register) (V:=Word) r q w)
-  (at level 20, q at level 50, format "r  ↦ᵣ{ q }  w") : bi_scope.
-Notation "r ↦1ᵣ w" := (mapsto (L:=Register) (V:=Word) r (DfracOwn 1) w) (at level 20) : bi_scope.
-Notation "r ↦2ᵣ w" := (mapsto (L:=Register) (V:=Word) r (DfracOwn 2) w) (at level 20) : bi_scope.
 
-(* Points to predicates for memory *)
-Notation "a ↦ₐ{ q } w" := (mapsto (L:=Addr) (V:=Word) a q w)
-  (at level 20, q at level 50, format "a  ↦ₐ{ q }  w") : bi_scope.
-Notation "a ↦1ₐ w" := (mapsto (L:=Addr) (V:=Word) a (DfracOwn 1) w) (at level 20) : bi_scope.
-Notation "a ↦2ₐ w" := (mapsto (L:=Addr) (V:=Word) a (DfracOwn 2) w) (at level 20) : bi_scope.
+Definition pointsto_mem1 `{!binDG Σ} (a : Addr) (q : Qp) (w : Word) :=
+    @pointsto Addr _ _ _ Σ fst_memG a (DfracOwn q) w.
+Definition pointsto_mem2 `{!binDG Σ} (a : Addr) (q : Qp) (w : Word) :=
+  @pointsto Addr _ _ _ Σ snd_memG a (DfracOwn q) w.
+
+Definition pointsto_reg1 `{!binDG Σ} (r : Register) (q : Qp) (w : Word) :=
+  @pointsto Register _ _ _ Σ fst_regG r (DfracOwn q) w.
+Definition pointsto_reg2 `{!binDG Σ} (r : Register) (q : Qp) (w : Word) :=
+  @pointsto Register _ _ _ Σ snd_regG r (DfracOwn q) w.
+
+(* First register *)
+Notation "r ↦1ᵣ{ q } w" := (pointsto_reg1 r q w)
+                              (at level 20, q at level 50, format "r  ↦1ᵣ{ q }  w") : bi_scope.
+Notation "r ↦1ᵣ w" :=
+    (pointsto_reg1 r 1 w) (at level 20) : bi_scope.
+Notation "r ↦1ᵣ{ q } -" := (∃ w, r ↦1ᵣ{q} w)%I
+                              (at level 20, q at level 50, format "r  ↦1ᵣ{ q }  -") : bi_scope.
+Notation "l ↦1ᵣ -" := (l ↦1ᵣ{1} -)%I (at level 20) : bi_scope.
+
+(* Second register *)
+Notation "r ↦2ᵣ{ q } w" := (pointsto_reg2 r q w)
+                             (at level 20, q at level 50, format "r  ↦2ᵣ{ q }  w") : bi_scope.
+Notation "r ↦2ᵣ w" :=
+  (pointsto_reg2 r 1 w) (at level 20) : bi_scope.
+Notation "r ↦2ᵣ{ q } -" := (∃ w, r ↦2ᵣ{q} w)%I
+                             (at level 20, q at level 50, format "r  ↦2ᵣ{ q }  -") : bi_scope.
+Notation "l ↦2ᵣ -" := (l ↦2ᵣ{1} -)%I (at level 20) : bi_scope.
+
+(* First memory *)
+Notation "r ↦1ₐ{ q } w" := (pointsto_mem1 r q w)
+                             (at level 20, q at level 50, format "r  ↦1ₐ{ q }  w") : bi_scope.
+Notation "r ↦1ₐ w" :=
+  (pointsto_mem1 r 1 w) (at level 20) : bi_scope.
+Notation "r ↦1ₐ{ q } -" := (∃ w, r ↦1ₐ{q} w)%I
+                             (at level 20, q at level 50, format "r  ↦1ₐ{ q }  -") : bi_scope.
+Notation "l ↦1ₐ -" := (l ↦1ₐ{1} -)%I (at level 20) : bi_scope.
+
+(* Second memory *)
+Notation "r ↦2ₐ{ q } w" := (pointsto_mem2 r q w)
+                             (at level 20, q at level 50, format "r  ↦2ₐ{ q }  w") : bi_scope.
+Notation "r ↦2ₐ w" :=
+  (pointsto_mem2 r 1 w) (at level 20) : bi_scope.
+Notation "r ↦2ₐ{ q } -" := (∃ w, r ↦2ₐ{q} w)%I
+                             (at level 20, q at level 50, format "r  ↦2ₐ{ q }  -") : bi_scope.
+Notation "l ↦2ₐ -" := (l ↦2ₐ{1} -)%I (at level 20) : bi_scope.
 
 Lemma wp_halt pc prog ll E Φ :
     prog pc = Halt ->
